Using the machinery for dependency discovery for the Liquidity extraction. Fixes some issues with type deboxing. Changed printing of fixpoins in Liquidity.

extraction/examples/CounterCertifiedExtraction.v
@@ -1,12 +1,15 @@
 From Coq Require Import PeanoNat ZArith Notations.
 
 From MetaCoq.Template Require Import Loader.
+From MetaCoq.Erasure Require Import Loader.
 
 From ConCert.Embedding Require Import MyEnv CustomTactics.
 From ConCert.Embedding Require Import Notations.
 From ConCert.Embedding Require Import SimpleBlockchain.
-From ConCert.Extraction Require Import LPretty Certified.
-
+From ConCert.Extraction Require Import LPretty LiquidityExtract Common Optimize PreludeExt.
+From ConCert.Execution Require Import Automation.
+From ConCert.Execution Require Import Serializable.
+From ConCert.Execution Require Import Blockchain.
 From Coq Require Import List Ascii String.
 Local Open Scope string_scope.
 
@@ -22,9 +25,18 @@ Definition PREFIX := "".
 
 Module Counter.
 
+  (** Enabling recursors for records allows for deriving [Serializable] instances. *)
+  Set Nonrecursive Elimination Schemes.
+
+  (** The definitions in this section are generalized over the [ChainBase] that specifies the type of addresses and which properties such a type must have *)
   Notation address := nat.
 
+  Definition operation := ActionBody.
   Definition storage := Z × address.
+
+  Definition init (ctx : SimpleCallCtx) (setup : Z * address) : option storage :=
+    let ctx' := ctx in (* prevents optimisations from removing unused [ctx]  *)
+    Some setup.
 
   Inductive msg :=
   | Inc (_ : Z)
@@ -37,17 +49,62 @@ Module Counter.
     (st.1 - new_balance, st.2).
 
   Definition counter (msg : msg) (st : storage)
-    : option (list SimpleActionBody_coq * storage) :=
+    : option (list operation * storage) :=
     match msg with
     | Inc i =>
       if (0 <=? i) then
-        Some ([], inc_balance st i)
+        Some ([],inc_balance st i)
       else None
     | Dec i =>
       if (0 <=? i) then
-        Some ([], dec_balance st i)
+        Some ([],dec_balance st i)
       else None
     end.
+
+  Definition COUNTER_MODULE : LiquidityMod msg _ (Z × address) storage operation :=
+  {| (* a name for the definition with the extracted code *)
+     lmd_module_name := "liquidity_counter" ;
+
+     (* definitions of operations on pairs and ints *)
+     lmd_prelude := prod_ops ++ nl ++ int_ops;
+
+     (* initial storage *)
+     lmd_init := init ;
+
+     (* no extra operations in [init] are required *)
+     lmd_init_prelude := "" ;
+
+     (* the main functionality *)
+     lmd_receive := counter ;
+
+     (* code for the entry point *)
+     lmd_entry_point := printWrapper (PREFIX ++ "counter") ++ nl
+                       ++ printMain |}.
+
+
+
+  (** These definitions define a contract in a format required by the execution framework. Note that these definitions will not be used for extraction. We extract the definitions above instead. *)
+  Definition counter_init (ch : Chain) (ctx : ContractCallContext) :=
+    init_wrapper init ch ctx.
+
+          Definition counter_receive (chain : Chain) (ctx : ContractCallContext)
+                     (st : storage) (msg : option msg) : option (storage * list ActionBody)
+            := match msg with
+               | Some m => match counter m st with
+                          | Some res => Some (res.2,res.1)
+                          | None => None
+                          end
+               | None => None
+               end.
+
+          (** Deriving the [Serializable] instances for the state and for the messages *)
+          Global Instance Msg_serializable : Serializable msg :=
+            Derive Serializable msg_rect<Inc, Dec>.
+
+  (** A contract instance used by the execution framework *)
+  Program Definition CounterContract :=
+    build_contract counter_init _ counter_receive _.
+  Next Obligation. easy. Qed.
 
 End Counter.
 
@@ -81,60 +138,39 @@ Qed.
 
 Import Counter.
 
-Definition local_def := local PREFIX.
+(** A translation table for definitions we want to remap. The corresponding top-level definitions will be *ignored* *)
+Definition TT_remap : list (kername * string) :=
+  [ remap <% bool %> "bool"
+  ; remap <% list %> "list"
+  ; remap <% Amount %> "tez"
+  ; remap <% address_coq %> "address"
+  ; remap <% time_coq %> "timestamp"
+  ; remap <% option %> "option"
+  ; remap <% Z.add %> "addInt"
+  ; remap <% Z.sub %> "subInt"
+  ; remap <% Z.leb %> "leInt"
+  ; remap <% Z %> "int"
+  ; remap <% nat %> "key_hash" (* type of account addresses*)
+  ; remap <% operation %> "operation"
+  ; remap <% @fst %> "fst"
+  ; remap <% @snd %> "snd" ].
 
-(** A translation table for various constants we want to rename *)
-Definition TT : env string :=
-  [  remap <% Z.add %> "addInt"
-     ; remap <% Z.sub %> "subInt"
-     ; remap <% Z.leb %> "leInt"
-     ; remap <% Z %> "int"
-     ; remap <% nat %> "address"
-     ; ("Some", "Some")
-     ; ("None", "None")
-     ; ("Z0" ,"0")
-     ; ("nil", "[]")
-     ; remap <% @fst %> "fst"
-     ; remap <% @snd %> "snd"
-     ; remap <% storage %> "storage"
-     ; local_def <% storage %>
-     ; local_def <% option %>
-     ; local_def <% msg %>
-     ; local_def <% inc_balance %>
-     ; local_def <% dec_balance %>
-  ].
+(** A translation table of constructors and some constants. The corresponding definitions will be extracted and renamed. *)
+Definition TT_rename :=
+  [ ("Some", "Some")
+  ; ("None", "None")
+  ; ("Z0" ,"0")
+  ; ("nil", "[]") ].
 
-MetaCoq Quote Recursively Definition counter_syn := (unfolded counter).
+(* Time Eval vm_compute in (erase_and_check_applied counter_syn). *)
 
-Time Eval vm_compute in (erase_and_check_applied counter_syn).
+(* TODO : revisit the description after proofs for deboxing are done *)
+(** We run the extraction procedure inside the [TemplateMonad]. It uses the certified erasure from [MetaCoq] and (so far uncertified) de-boxing procedure that removes application of boxes to constants and constructors. *)
 
-(** We run the extraction procedure inside the [TemplateMonad]. It uses the certified erasure from [MetaCoq] and (so far uncertified) de-boxing procedure that removes application of boxes to constants and constructors. Even though the de-boxing is not certified yet, before removing boxes we check if constant is applied to all logical argument (i.e. proofs or types) and constructors are fully applied. In this case, it is safe to remove these applications. *)
 Time MetaCoq Run
-    (storage_def <- tmQuoteConstant <%% storage %%> false ;;
-     storage_body <- opt_to_template storage_def.(cst_body) ;;
-     ind <- tmQuoteInductive <%% msg %%> ;;
-     ind_liq <- print_one_ind_body PREFIX TT ind.(ind_bodies);;
-     t1 <- toLiquidity PREFIX TT inc_balance ;;
-     t2 <- toLiquidity PREFIX TT dec_balance ;;
-     t3 <- toLiquidity PREFIX TT counter ;;
-     res <- tmEval lazy
-                  (prod_ops ++ nl ++ int_ops
-                     ++ nl ++ nl
-                     ++ "type storage = " ++ print_liq_type PREFIX TT storage_body
-                     ++ nl ++ nl
-                     ++ ind_liq
-                     ++ nl ++ nl
-                     ++ t1
-                     ++ nl ++ nl
-                     ++ t2
-                     ++ nl ++ nl
-                     ++ t3
-                     ++ nl ++ nl
-                     ++ printWrapper (PREFIX ++ "counter")
-                     ++ nl ++ nl
-                     ++ printMain) ;;
-    tmDefinition "counter_extracted" res).
+     (t <- liquitidy_extraction PREFIX TT_remap TT_rename COUNTER_MODULE ;;
+      tmDefinition COUNTER_MODULE.(lmd_module_name) t).
 
-Print counter_extracted.
+Print liquidity_counter.
 
-Redirect "counter.liq" Print counter_extracted.
+Redirect "counter.liq" Print liquidity_counter.
