extraction/examples/CrowdfundingCertifiedExtraction.v
@@ -2,7 +2,7 @@ Require Import String ZArith Basics.
 From ConCert.Embedding Require Import Ast Notations CustomTactics
      PCUICTranslate PCUICtoTemplate Utils MyEnv.
 
-From ConCert.Extraction Require Import Certified LPretty.
+From ConCert.Extraction Require Import LiquidityExtract LPretty Common.
 From ConCert.Extraction.Examples Require Import PreludeExt CrowdfundingData Crowdfunding SimpleBlockchainExt.
 
 From Coq Require Import List Ascii String.
@@ -22,80 +22,96 @@ Import Receive.
 
 Definition PREFIX := "".
 
-Definition local_def := local PREFIX.
-
-(** A translation table for various constants we want to rename *)
-Definition TT : env string :=
+(** A translation table for definitions we want to remap. The corresponding top-level definitions will be *ignored* *)
+Definition TT_remap : list (kername * string) :=
   [  (* types *)
-       remap <% Z %> "tez"
-     ; remap <% address_coq %> "address"
-     ; remap <% time_coq %> "timestamp"
-     ; remap <% nat %> "nat"
-     ; remap <% bool %> "bool"
-     ; remap <% unit %> "unit"
-     ; remap <% list %> "list"
-     ; remap <% @fst %> "fst"
-     ; remap <% @snd %> "snd"
-     ; remap <% option %> "option"
-     ; remap <% Maps.addr_map_coq %> "(address,tez) map"
-     ; remap <% SimpleActionBody_coq %> "operation"
+    remap <% Z %> "tez"
+  ; remap <% address_coq %> "address"
+  ; remap <% time_coq %> "timestamp"
+  ; remap <% nat %> "nat"
+  ; remap <% bool %> "bool"
+  ; remap <% unit %> "unit"
+  ; remap <% list %> "list"
+  ; remap <% @fst %> "fst"
+  ; remap <% @snd %> "snd"
+  ; remap <% option %> "option"
+  ; remap <% Maps.addr_map_coq %> "(address,tez) map"
+  ; remap <% SimpleActionBody_coq %> "operation"
 
-     ; remap <% Z.add %> "addTez"
-     ; remap <% Z.eqb %> "eqTez"
-     ; remap <% Z.leb %> "leTez"
-     ; remap <% Z.ltb %> "ltTez"
-     ; remap <% ltb_time %> "ltb_time"
-     ; remap <% leb_time %> "leb_time"
-     ; remap <% eqb_addr %> "eq_addr"
-     ; remap <% andb %> "andb"
-     ; remap <% negb %> "not"
-     ; remap <% Maps.add_map %> "Map.add"
-     ; remap <% lookup_map' %> "Map.find"
+  (* operations *)
+  ; remap <% Z.add %> "addTez"
+  ; remap <% Z.eqb %> "eqTez"
+  ; remap <% Z.leb %> "leTez"
+  ; remap <% Z.ltb %> "ltTez"
+  ; remap <% ltb_time %> "ltb_time"
+  ; remap <% leb_time %> "leb_time"
+  ; remap <% eqb_addr %> "eq_addr"
+  ; remap <% andb %> "andb"
+  ; remap <% negb %> "not"
+  ; remap <% Maps.add_map %> "Map.add"
+  ; remap <% lookup_map' %> "Map.find" ].
 
-     ; ("Z0" ,"0DUN")
-     ; ("nil", "[]")
-     ; ("tt", "()")
-
-     ; local_def <% msg_coq %>
-
-     ; local_def <% update_contribs %>
-     ; local_def <% maybe_bind_unit %>
-     ; local_def <% set_done %>
-     ; local_def <% validate %>
-  ].
-
+(** A translation table of constructors and some constants. The corresponding definitions will be extracted and renamed. *)
+Definition TT_rename :=
+  [ ("Z0" ,"0DUN")
+  ; ("nil", "[]")
+  ; ("mnil", "Map []")
+  ; ("tt", "()") ].
 
 Definition printWrapperAndMain :=
   "let wrapper (msg : msg_coq)(st : ((timestamp * (tez * address)) * ((address,tez) map * bool))) = match receive msg st (Current.time (), (Current.sender (), (Current.amount (), Current.balance ()))) with
-| Some v -> v| None -> failwith ()
-let%entry main (msg : msg_coq)(st : ((timestamp * (tez * address)) * ((address,tez) map * bool))) = wrapper msg st".
+| Some v -> v| None -> failwith ()" ++ nl ++ nl++
+"let%entry main (msg : msg_coq)(st : ((timestamp * (tez * address)) * ((address,tez) map * bool))) = wrapper msg st".
+
+
+Notation storage := ((time_coq × Z × address_coq) × Maps.addr_map_coq × bool).
+Notation params := ((time_coq × address_coq × Z × Z) × msg_coq).
+Definition crowdfunding_init (ctx : SimpleCallCtx)
+           (setup : (time_coq × Z × address_coq)) : option storage :=
+  if ctx.2.2.1 =? 0 then Some (setup, (Maps.mnil, false)) else None.
+  (* (unfolded Init.init) setup ctx. *)
+
+Definition crowdfunding_receive
+           (params : params)
+           (st : storage) : option (list SimpleActionBody_coq × storage) :=
+  receive params.2 st params.1.
+
+Definition COUNTER_MODULE :
+  LiquidityMod params SimpleCallCtx (time_coq × Z × address_coq) storage SimpleActionBody_coq :=
+  {| (* a name for the definition with the extracted code *)
+     lmd_module_name := "liquidity_crowdfunding" ;
+
+     (* definitions of operations on pairs and ints *)
+     lmd_prelude :=
+       LiquidityPrelude
+         ++ nl
+         ++ "type storage = ((timestamp * (tez * address)) * ((address,tez) map * bool))";
+
+     (* initial storage *)
+     lmd_init := crowdfunding_init ;
+
+     (* init requires some extra operations *)
+     lmd_init_prelude :=
+            "let fst (p : 'a * 'b) : 'a = p.(0) in"
+         ++ nl
+         ++ "let snd (p : 'a * 'b) : 'b = p.(1) in"
+         ++ nl
+         ++ "let eqTez (a : tez ) (b : tez ) = a = b in" ;
+
+
+     (* the main functionality *)
+     lmd_receive := crowdfunding_receive  ;
+
+     (* code for the entry point *)
+     lmd_entry_point := printWrapperAndMain |}.
+
+
+(* TODO : revisit the description after proofs for deboxing are done *)
+(** We run the extraction procedure inside the [TemplateMonad]. It uses the certified erasure from [MetaCoq] and (so far uncertified) de-boxing procedure that removes application of boxes to constants and constructors. *)
 
 Time MetaCoq Run
-     (ind <- tmQuoteInductive <%% msg_coq %%> ;;
-     ind_liq <- print_one_ind_body PREFIX TT ind.(ind_bodies);;
-     t1 <- toLiquidity PREFIX TT update_contribs ;;
-     t2 <- toLiquidity PREFIX TT maybe_bind_unit ;;
-     t3 <- toLiquidity PREFIX TT set_done ;;
-     t4 <- toLiquidity PREFIX TT validate ;;
-     t5 <- toLiquidity PREFIX TT receive ;;
-     res <- tmEval lazy
-                  (LiquidityPrelude
-                     ++ nl ++ nl
-                     ++ "type storage = ((timestamp * (tez * address)) * ((address,tez) map * bool))"
-                     ++ nl ++ nl
-                     ++ ind_liq
-                     ++ nl ++ nl
-                     ++ t1
-                     ++ nl ++ nl
-                     ++ t2
-                     ++ nl ++ nl
-                     ++ t3
-                     ++ nl ++ nl
-                     ++ t4
-                     ++ nl ++ nl
-                     ++ t5
-                     ++ nl ++ nl
-                     ++ printWrapperAndMain ) ;;
-    tmDefinition "crowdfunding_extracted" res).
+     (t <- liquitidy_extraction PREFIX TT_remap TT_rename COUNTER_MODULE ;;
+      tmDefinition COUNTER_MODULE.(lmd_module_name) t
+     ).
 
-Print crowdfunding_extracted.
+Print liquidity_crowdfunding.
