extraction/examples/StackInterpreter.v
@@ -7,9 +7,9 @@ From MetaCoq.PCUIC Require Import TemplateToPCUIC PCUICTyping.
 
 From ConCert Require Import MyEnv.
 From ConCert.Embedding Require Import Notations.
-From ConCert.Embedding Require Import SimpleBlockchain.
-From ConCert.Extraction Require Import LPretty Certified Extra Erasure Common.
-From ConCert.Execution Require Import Containers.
+From ConCert.Extraction Require Import LPretty LiquidityExtract
+     Erasure Common PreludeExt.
+From ConCert.Execution Require Import Containers Blockchain.
 
 From Coq Require Import List Ascii String.
 Local Open Scope string_scope.
@@ -21,11 +21,8 @@ Import MonadNotation.
 
 Definition PREFIX := "".
 
-(** Quoting this runs forever, because of many dependencies *)
-Definition lookup (m : FMap string Z) (k : string) := FMap.find k m.
-(* Quote Recursively Definition lookup_quoted :=lookup. *)
-
 Definition map_key_type := (string * Z).
+Definition action := ActionBody.
 
 Module Interpreter.
 
@@ -43,6 +40,10 @@ Module Interpreter.
   Definition lookup (k : string * Z) (m : ext_map) := FMap.find k m.
 
   Definition storage := list value.
+
+  Definition init (ctx : SimpleCallCtx) (setup : unit) : option storage :=
+    let ctx' := ctx in (* prevents optimisations from removing unused [ctx]  *)
+    Some [].
 
   Definition params := list instruction * ext_map.
 
@@ -76,280 +77,80 @@ Module Interpreter.
       end
     end.
 
-  Definition receive (p : params) (s : list value) := interp p.2 p.1 s.
+  Definition receive (p : params) (s : list value)
+    : option (list action * storage) :=
+    let s' := s in (* prevents optimisations from removing unused [s]  *)
+    match interp p.2 p.1 [] with
+    | Some v => Some ([],v)
+    | None => None
+    end.
 
 End Interpreter.
 
-(* Erase the unignored global declarations by the specified names and
-   their non-erased dependencies recursively. *)
-(* Fixpoint q_rec *)
-(*         (Σ : P.global_env) *)
-(*         (ignored : list kername) *)
-(*         (include : list kername): global_env:= *)
-(*   match Σ with *)
-(*   | [] => [] *)
-(*   | (kn, decl) :: Σ => *)
-(*     if contains kn include && negb (contains kn ignored)  then *)
-(*       (kn, decl) :: q_rec Σ ignored (decl_deps include decl) *)
-(*     else *)
-(*       q_rec Σ _ include *)
-(*   end. *)
-(* Next Obligation. now sq; inversion wfΣ. Qed. *)
-(* Next Obligation. now sq; inversion wfΣ. Qed. *)
-(* Next Obligation. now sq; inversion wfΣ. Qed. *)
-(* Next Obligation. now sq; inversion wfΣ. Qed. *)
-
-
-(* Import Interpreter. *)
-(* Input for the interpreter in Liquidity:
-
-([IPushZ 0; IObs ("blah",0); IOp Add; IPushZ 1; IOp Equal], (Map [(("blah", 0), (ZVal 1))])) *)
-(* Example test_interp : *)
-(*   let env  := FMap.of_list [(("blah", 0%Z), (ZVal 1))] in *)
-(*   interp env [IPushZ 0; IObs "blah" 0; IOp Add; IPushZ 1; IOp Equal] [] = Some [BVal true]. *)
-(* Proof. reflexivity. Qed. *)
-
-Module Interpreter1.
-
-  Inductive op : Set := Add | And | Equal.
-
-  Inductive instruction :=
-  | IPushZ : Z -> instruction
-  | IPushB : bool -> instruction
-  | IOp : op -> instruction.
-
-  Inductive value : Set := BVal : bool -> value | ZVal : Z -> value.
-
-  Definition storage := list value.
-
-  Definition params := list instruction.
-
-  Fixpoint interp (insts : list instruction) (s : list value) :=
-    match insts with
-    | [] => Some s
-    | hd :: inst' =>
-      match hd with
-      | IPushZ i => interp inst' (ZVal i :: s)
-      | IPushB b => interp inst' (BVal b :: s)
-      | IOp op => match op with
-                   | Add => match s with
-                            | ZVal i :: ZVal j :: s' => interp inst' (ZVal (i+j) :: s')%Z
-                            | _ => None
-                            end
-                   | And => match s with
-                            | BVal i :: BVal j :: s' => interp inst' (BVal (i && j) :: s')%Z
-                            | _ => None
-                           end
-                   | Equal => match s with
-                            | ZVal i :: ZVal j :: s' => interp inst' (BVal (i =? j) :: s')%Z
-                            | _ => None
-                             end
-                 end
-      end
-    end.
-
-  Definition receive (p : params) (s : list value) := interp p s.
-
-End Interpreter1.
-
-
 Import Interpreter.
 
-Definition local_def := local PREFIX.
+(** Input for the interpreter in Liquidity: *)
+(** ([IPushZ 0; IObs ("blah",0); IOp Add; IPushZ 1; IOp Equal], (Map [(("blah", 0), (ZVal 1))])) *)
+Example test_interp :
+  let env  := FMap.of_list [(("blah", 0%Z), (ZVal 1))] in
+  interp env [IPushZ 0; IObs "blah" 0; IOp Add; IPushZ 1; IOp Equal] [] =
+  Some [BVal true].
+Proof. reflexivity. Qed.
 
 Definition print_finmap_type (prefix ty_key ty_val : string) :=
   parens false (ty_key ++ "," ++ prefix ++ ty_val) ++ " map".
 
 (** A translation table for various constants we want to rename *)
-Definition TT_remap : MyEnv.env string :=
+Definition TT_remap : list (kername * string) :=
   [   (* remapping types *)
        remap <% Z %> "int"
      ; remap <% bool %> "bool"
-     ; remap <% nat %> "address"
+     ; remap <% unit %> "unit"
+     ; remap <% option %> "option"
+     ; remap <% Amount %> "tez"
+     ; remap <% address_coq %> "address"
+     ; remap <% time_coq %> "timestamp"
      ; remap <% list %> "list"
      ; remap <% string %> "string"
      ; remap <% ext_map %> (print_finmap_type PREFIX "string * int" "value")
+     ; remap <% action %> "operation"
      (* remapping operations *)
      ; remap <% Z.add %> "addInt"
      ; remap <% Z.eqb %> "eqInt"
      ; remap <% @lookup %> "Map.find"
      ; remap <% @fst %> "fst"
      ; remap <% @snd %> "snd"
-     ; remap <% andb %> "andb"
+       ; remap <% andb %> "andb" ].
 
-     (* remapping constructors *)
-     ; ("Some", "Some")
-     ; ("None", "None")
-     ; ("true", "true")
-     ; ("false", "false")
+Definition TT_rename : MyEnv.env string :=
+     (* constructors *)
+     [ ("Z0" ,"0")
+     ; ("nil", "[]")].
 
-     ; ("Z0" ,"0")
-     ; ("nil", "[]") ].
-
-Definition TT_remap_names  :=
-  [
-       <%% Z %%>
-     ; <%% bool %%>
-     ; <%% nat %%>
-     ; <%% list %%>
-     ; <%% string %%>
-     ; <%% ext_map %%>
-     ; <%% Z.add %%>
-     ; <%% Z.eqb %%>
-     ; <%% @fst %%>
-     ; <%% @snd %%>
-     ; <%% andb %%>
-     ; <%% @lookup %%>].
-
-
-Definition TT_local :=
-    (* local types *)
-  [    local_def <% storage %>
-     ; local_def <% params %>
-     ; local_def <% interp %>
-     ; local_def <% instruction %>
-     ; local_def <% value %>
-     ; local_def <% op %>].
-
-Definition TT := (TT_remap ++ TT_local)%list.
-
-(** A wrapper for calling the main functionality [func_name]. It is important to be explicit about types for all the parameters of entry points *)
-Definition print_main (func_name : string): string :=
-  let func_name := PREFIX ++ func_name in
-  let params_name := PREFIX ++ "params" in
-  "let%entry main (p : " ++ params_name ++ ")" ++ " s ="
-    ++ nl
-    ++ "match " ++ func_name ++ " p []"  ++ " with"
-    ++ nl
-    ++ "| Some res -> ( [], res ) "
-    ++ nl
-    ++ "| _ -> Current.failwith s".
-
-Fixpoint combine_global_envs (Σ Σ' : global_env) : global_env :=
-  match Σ' with
-  | [] => Σ
-  | (nm,d) :: Σ'' => match (lookup_env Σ nm) with
-                   | Some _ => (combine_global_envs Σ Σ'')%list
-                   | None => ((nm,d) :: combine_global_envs Σ Σ'')%list
-                   end
-  end.
-
-Definition INTERP_MODULE : LiquidityModule :=
+Definition INTERP_MODULE : LiquidityMod params _ _ storage action :=
   {| (* a name for the definition with the extracted code *)
-     lm_module_name := "liquidity_interp" ;
+     lmd_module_name := "liquidity_interp" ;
 
      (* definitions of operations on ints, bools, pairs, ect. *)
-     lm_prelude := prod_ops ++ nl ++ int_ops ++ nl ++ bool_ops;
+     lmd_prelude := prod_ops ++ nl ++ int_ops ++ nl ++ bool_ops;
 
-     (* inductives -- in the order that respect dependency *)
-     lm_adts := [<%% op %%>;<%% instruction %%>;<%% value %%>];
+     lmd_init := init ;
 
-     (* definitions: type abbreviations and functions -- in the order that respect dependency *)
-     (* lm_defs := [<%% params %%>; <%% storage %%>; *)
-     (*                 <%% obs0 %%>; *)
-     (*                 <%% interp %%>; <%% receive %%>]; *)
-     lm_defs := [<%% params %%>;<%% receive %%>] ;
+     lmd_init_prelude := "";
+
+     lmd_receive := receive ;
 
      (* code for the entry point *)
-     lm_entry_point := print_main "receive";
+     lmd_entry_point :=
+           printWrapper (PREFIX ++ "receive")
+                        ++ nl
+                        ++ printMain |}.
 
-     (* initial storage *)
-     lm_init := "[]" |}.
-
-(** Adds a definition containing a global environment containing all dependencies required for erasure *)
-
-Time MetaCoq Run (t <- tmQuoteRecTransp Interpreter.receive false ;;
-             tmDefinition "GE" t.1).
-
-Compute (List.length GE).
-
-(* Time Compute (specialize_erase_debox_template_env GE [<%% interp %%>] TT_remap_names ). *)
-
-(* Metacoq Run (ps <- monad_map erasable_program (List.rev INTERP_MODULE.(lm_defs)) ;; *)
-(*              (* let env := fold_left combine_global_envs (map rev (map (fst) ps)) [] in *) *)
-(*              let env := List.concat (map (fst) ps) in *)
-(*              res <- tmEval all env ;; *)
-(*              tmDefinition "GE" res). *)
-(* Compute GE. *)
-
-Definition clear_bodies (Σ : global_env) :=
-  map (fun '(kn,gd) => (kn, match gd with
-                         | ConstantDecl c => ConstantDecl
-                                              (Build_constant_body
-                                                 c.(cst_type)
-                                                 None
-                                                 c.(cst_universes))
-                         | _ => gd
-                         end)) Σ.
-
-Definition GE' := List.filter (fun '(n, _) => negb (eq_kername n <%% interp %%> )%string) GE.
-
-Import ResultMonad.
-
-Definition e_glob_dec Σ :=
-  match erase_global_decls TT_remap_names Σ (todo "") with
-  | Err c => inr (string_of_erase_global_decl_error c)
-  | Ok e => inl e
-  end.
-
-Definition e_glob_dec_rec Σ seeds :=
-  match erase_global_decls_deps_recursive TT_remap_names Σ (todo "") seeds with
-  | Err c => inr (string_of_erase_global_decl_error c)
-  | Ok e => inl e
-  end.
-
-Time MetaCoq Run (
-         Σ' <- tmEval lazy (Tglobal_decls_deps_recursive TT_remap_names GE [<%% receive %%>]) ;;
-         tmDefinition "GE_interp" Σ').
-
-Compute List.length GE_interp.
-
-Definition GE_interp' := List.filter (fun '(n, _) => negb (eq_kername n <%% ext_map %%> )%string) GE_interp.
-
-Compute List.length GE_interp'.
-
-(* Succeeds *)
-Time Compute (let Σ := (trans_global (Ast.empty_ext GE_interp)).1 in
-              e_glob_dec Σ).
-
-(* Fails and complains about dependencies *)
-Compute (
-    let Σ := (trans_global (Ast.empty_ext GE_interp)).1 in
-    e_glob_dec_rec Σ [<%% interp %%>]).
-
-Compute (specialize_erase_debox_template_env GE_interp [<%% interp %%>] TT_remap_names).
-
-(* Hangs forever *)
-Compute (specialize_erase_debox_template_env GE [<%% interp %%>] TT_remap_names).
-
-
-(* Hangs forever*)
-(* Compute ( *)
-(*     let Σ := (trans_global (Ast.empty_ext GE)).1 in *)
-(*     SafeErasureFunction.erase_global Σ (todo "")). *)
-
-
-Time Compute (let Σ := (trans_global (Ast.empty_ext (firstn 182 GE))).1 in
-          e_glob_dec Σ).
-
-Time MetaCoq Run (
-       c <- tmQuoteConstant <%% interp %%> false ;;
-       print_nf (erase_print_deboxed_all_applied "" TT (clear_bodies GE) <%% interp %%> c)).
-(*           ). *)
-(* MetaCoq Run ( *)
-(*           let GE' := List.filter (fun '(n, _) => negb (eq_kername n <%% interp %%> )%string) GE in *)
-(*           let Σ := (trans_global (Ast.empty_ext GE')).1 in *)
-(*           p <- tmQuoteConstant <%% interp %%> false;; *)
-(*           let pp := (trans_constant_body p) in *)
-(*           match erase_constant_decl (P.empty_ext Σ) (todo "") pp (todo "") with *)
-(*           | ResultMonad.Ok t1 => *)
-(*             let GE' := (GE' ++ [(<%%interp%%>,ConstantDecl t1)])%list in *)
-(*             print_nf GE' *)
-(*             (* tmDefinition "GE'" (GE' ++ [(<%%interp%%>,t1)])%list *) *)
-(*           | ResultMonad.Err e => print_nf e *)
-(*           end). *)
 (** We translate required definitions and print them into a single string containing the whole program. The definition with the corresponding code is added to Coq's environment. *)
-Time MetaCoq Run (printLiquidityModule PREFIX GE TT INTERP_MODULE).
+Time MetaCoq Run
+     (t <- liquitidy_extraction PREFIX TT_remap TT_rename INTERP_MODULE ;;
+      tmDefinition INTERP_MODULE.(lmd_module_name) t
+     ).
 
 (** The extracted program can be printed and copy-pasted to the online Liquidity editor *)
 Print liquidity_interp.
