extraction/theories/Common.v
@@ -12,7 +12,7 @@ From MetaCoq Require Import MCSquash.
 From MetaCoq.Erasure Require Import EAst.
 From MetaCoq.Erasure Require Import SafeErasureFunction.
 From MetaCoq.Erasure Require Import SafeTemplateErasure.
-From MetaCoq.PCUIC Require Import PCUICAst.
+From MetaCoq.PCUIC Require Import PCUICAst PCUICTyping PCUICValidity TemplateToPCUIC.
 From MetaCoq.SafeChecker Require Import PCUICSafeChecker.
 From MetaCoq.SafeChecker Require Import SafeTemplateChecker.
 From MetaCoq.Template Require Import Ast.
@@ -25,6 +25,7 @@ From ConCert.Execution Require Import Serializable.
 From ConCert.Extraction Require Import Erasure.
 From ConCert.Extraction Require Import ResultMonad.
 From ConCert.Extraction Require Import StringExtra.
+From ConCert.Extraction Require Import Optimize.
 
 Module T := MetaCoq.Template.Ast.
 Module P := MetaCoq.PCUIC.PCUICAst.
@@ -428,16 +429,37 @@ Definition specialize_ChainBase_and_check
 
    After the environment has been specialized the dependencies of the
    specified seeds are recursively erased and deboxed, except for
-   names in the 'ignored' list, whose decls are ignored. The result is
+   names for which [ignore] returns [true], whose decls are ignored. The result is
    returned in proper topological order. Assumption: the global
    environment type checks. *)
+Definition general_specialize_erase_debox_template_env
+           (Σ : T.global_env)
+           (seeds : list kername)
+           (ignore : kername -> bool) : result ExAst.global_env string :=
+  '(Σ; wfΣ) <- specialize_ChainBase_and_check Σ;;
+  let ignored_names := filter ignore (map fst Σ) in
+  Σ' <- map_error string_of_erase_global_decl_error
+                 (general_erase_global_decls_deps_recursive Σ wfΣ ignore seeds) ;;
+  let mask := get_dearg_set_for_unused_args Σ' in
+  ret (debox_types_global_env (remove_unused_args mask Σ')).
+
+(* Like above, but takes a list of names to ignore *)
 Definition specialize_erase_debox_template_env
            (Σ : T.global_env)
            (seeds : list kername)
            (ignored : list kername) : result ExAst.global_env string :=
+  general_specialize_erase_debox_template_env Σ seeds (fun kn => contains kn ignored).
+
+(* Like above, but does not debox *)
+Definition specialize_erase_template_env
+           (Σ : T.global_env)
+           (seeds : list kername)
+           (ignored : list kername) : result ExAst.global_env string :=
   '(Σ; wfΣ) <- specialize_ChainBase_and_check Σ;;
+  let ignore kn := contains kn ignored in
   map_error string_of_erase_global_decl_error
-            (erase_global_decls_deps_recursive ignored Σ wfΣ seeds).
+            (general_erase_global_decls_deps_recursive Σ wfΣ ignore seeds).
+
 
 (*
 (* Like above, but get the dependencies from the term of a template
@@ -542,4 +564,287 @@ Definition get_contract_extraction_set
   match specialize_erase_debox_template_env p.1 seeds ignored_concert_types with
   | Ok Σ => ret {| env := Σ; init_name := init_name; receive_name := receive_name; |}
   | Err err => tmFail err
+  end.
+
+(** Extracts a constant name, inductive name or returns None *)
+Definition to_kername (t : Ast.term) : option kername :=
+  match t with
+  | Ast.tConst c _ => Some c
+  | Ast.tInd c _ => Some c.(inductive_mind)
+  | _ => None
+  end.
+
+Definition to_kername_dummy (t : Ast.term) :  kername :=
+  let dummy := (MPfile [],"") in
+  match (to_kername t) with
+  | Some v => v
+  | None => dummy
+  end.
+
+Notation "<%% t %%>" := (to_kername_dummy <% t %>).
+
+Definition to_string_name (t : Ast.term) : string :=
+  match to_kername t with
+  | Some kn => string_of_kername kn
+  | None => "Not a constant or inductive"
+  end.
+
+Notation "'unfolded' d" :=
+  ltac:(let y := eval unfold d in d in exact y) (at level 100, only parsing).
+
+(** Returns a pair of a kername (if [t] is a constant) and a new name.
+ Used in a similar way as [Extract Inlined Constant] of the standard extraction *)
+Definition remap (t : Ast.term) (new_name : string) :  kername * string :=
+  let nm := to_kername_dummy t in
+  (nm, new_name).
+
+(** ** Validation of applied constants and constructors *)
+
+Definition is_fully_applied_ctor (Σ : P.global_env)
+           (ind : inductive)
+           (ctor : nat) (n_app : nat) :=
+  match PCUICChecker.lookup_constructor_decl Σ ind.(inductive_mind) ind.(inductive_ind) ctor with
+  | PCUICChecker.Checked (_,_,ty) =>
+    let (dom, _) :=
+        PCUICAstUtils.decompose_prod ty in
+    Nat.eqb n_app (List.length dom.2)
+  | _ => false
+  end.
+
+Definition find_indices {A : Type}
+           (f : A -> bool) : list A -> list nat :=
+  let worker := fix go (i : nat) l :=
+              match l with
+              | [] => []
+              | x :: tl =>
+                if f x then i :: go (1+i)%nat tl
+                else go (1+i)%nat tl
+              end in
+  worker 0.
+
+Fixpoint last_option {A} (l : list A) : option A :=
+  match l with
+  | [] => None
+  | [a] => Some a
+  | a :: (_ :: _) as l0 => last_option l0
+  end.
+
+Import ExAst.
+
+Definition is_TBox (t : box_type) : bool :=
+  match t with
+  | TBox => true
+  | _ => false
+  end.
+
+Definition last_box_index l := last_option (find_indices is_TBox l).
+
+Fixpoint lookup_env (Σ : P.global_env) (id : kername) : option P.global_decl :=
+  match Σ with
+  | nil => None
+  | hd :: tl =>
+    if eq_kername id hd.1 then Some hd.2
+    else lookup_env tl id
+  end.
+
+Definition lookup_ind_decl (Σ : P.global_env) ind i :=
+  match lookup_env Σ ind with
+  | Some (P.InductiveDecl {| P.ind_bodies := l; P.ind_universes := uctx |}) =>
+    match nth_error l i with
+    | Some body => Some body
+    | None => None
+    end
+  | _ => None
+  end.
+
+Definition lookup_const (Σ : P.global_env) const :=
+  match lookup_env Σ const with
+  | Some (P.ConstantDecl b) => Some b
+  | _ => None
+  end.
+
+Definition erase_type_to_typing_result {A} (e : erase_type_error) : typing_result A:=
+  match e with
+  | NotPrenex => TypeError (Msg "Not Prenex")
+  | TypingError te => TypeError te
+  | GeneralError msg => TypeError (Msg msg)
+  end.
+
+Program Fixpoint is_logargs_applied_const (Σ : P.global_env)
+           (HΣ : ∥ PCUICTyping.wf Σ ∥)
+           (const : kername) (n_app : nat) : typing_result bool :=
+  match Σ with
+  | (kn, P.ConstantDecl cst) :: Σ' =>
+    if eq_kername kn const then
+      let Σext := (Σ', universes_decl_of_decl (P.ConstantDecl cst)) in
+      match erase_type Σext _ [] Vector.nil cst.(P.cst_type) _ [] with
+      | ResultMonad.Ok ety =>
+        let (dom, _) := decompose_arr ety.2 in
+        match last_box_index dom with
+        | Some i => ret (Nat.leb (i+1) n_app)
+        | None => ret true
+        end
+      | ResultMonad.Err e => erase_type_to_typing_result e
+      end
+    else is_logargs_applied_const Σ' _ const n_app
+  | _ :: Σ' => is_logargs_applied_const Σ' _ const n_app
+  | _ => TypeError (Msg ("Constant not found: " ++ string_of_kername const))
+  end.
+Next Obligation. cbn;intros;subst; now sq; inversion HΣ. Qed.
+Next Obligation.
+  intros. sq.
+  unfold lookup_const in *. subst.
+  inversion HΣ;subst;cbn in *.
+  unfold on_constant_decl in *.
+  destruct (P.cst_body cst).
+  - cbn in X0.
+    eapply validity_term; [easy|exact X0].
+  - cbn in X0.
+    destruct X0 as (s & ?).
+    right.
+    now exists s.
+Qed.
+Next Obligation. cbn;intros;subst; now sq; inversion HΣ. Qed.
+Next Obligation. cbn;intros;subst; now sq; inversion HΣ. Qed.
+Next Obligation. cbn;intros;subst; now sq; inversion HΣ. Qed.
+Next Obligation. cbn;intros;subst; now sq; inversion HΣ. Qed.
+
+Program Definition test_applied_to_logargs  (p : Ast.program) (const : kername) (n_app : nat)
+  : EnvCheck bool :=
+  let p := fix_program_universes p in
+  let Σ := (trans_global (Ast.empty_ext p.1)).1 in
+  G <- check_wf_env_only_univs Σ ;;
+  t <- wrap_error (P.empty_ext Σ) "during cheking applied constant" (is_logargs_applied_const (P.empty_ext Σ) _ const n_app) ;;
+  ret (Monad:=envcheck_monad) t.
+Next Obligation.
+  intros.
+  unfold PCUICTyping.wf_ext, empty_ext.
+  unfold PCUICTyping.on_global_env_ext.
+  destruct G as (?&H&H0). now sq.
+Qed.
+
+MetaCoq Quote Recursively Definition ex_combine := combine.
+
+Example test_combine_true :
+  (test_applied_to_logargs ex_combine (to_kername_dummy <% @combine %>) 2)
+  =
+  CorrectDecl true.
+Proof. reflexivity. Qed.
+
+Example test_combine_false :
+  (test_applied_to_logargs ex_combine (to_kername_dummy <% @combine %>) 1)
+  =
+  CorrectDecl false.
+Proof. reflexivity. Qed.
+
+
+Definition test_fully_applied_constructor (p : Ast.program) (ind_nm : kername) (ind_i : nat) (ctor : nat) (n_app : nat) :=
+  let p := fix_program_universes p in
+  let Σ := (trans_global (Ast.empty_ext p.1)).1 in
+  (is_fully_applied_ctor Σ (mkInd ind_nm ind_i) ctor n_app).
+
+MetaCoq Quote Recursively Definition q_prod
+  := (fun (x y : nat) => (x,y)).
+
+Example test_pair_true :
+  (test_fully_applied_constructor q_prod (to_kername_dummy <% prod %>) 0 0 4)
+  = true.
+Proof. reflexivity. Qed.
+
+Example test_pair_false :
+  (test_fully_applied_constructor q_prod (to_kername_dummy <% prod %>) 0 0 3)
+  = false.
+Proof. reflexivity. Qed.
+
+
+Definition forallb_defs {A : Set} (f : A -> bool) (ds : list (E.def A)) :=
+  (* this way of defining is fixpoint-firendly, i.e. is we [map] first and then apply [forallb] it fails to work with the definition below *)
+  forallb (fun x => f x.(E.dbody)) ds.
+
+Open Scope bool.
+
+Definition check_ctors_applied (Σ : P.global_env) :=
+  fix go (apps : list E.term) (t : E.term) :=
+    match t with
+    | E.tRel i => true
+    | E.tEvar ev args => forallb (go []) args
+    | E.tLambda na M => go [] M
+    | E.tApp u v => (go (v :: apps) u) && (go [] v)
+    | E.tLetIn na b b' => (go [] b) && (go [] b')
+    | E.tCase ind c brs =>
+      let brs' := forallb (fun x => go [] (snd x)) brs in
+      (go [] c) && brs'
+    | E.tProj p c => go [] c
+    | E.tFix mfix idx =>
+      forallb_defs (go []) mfix
+    | E.tCoFix mfix idx =>
+      forallb_defs (go []) mfix
+    | E.tBox => true
+    | E.tVar _ => true
+    | E.tConst _ => true
+    | E.tConstruct ind i =>
+      is_fully_applied_ctor Σ ind i (List.length apps)
+    end.
+
+Definition check_consts_applied
+  (Σ : P.global_env_ext) (HΣ : ∥ PCUICTyping.wf Σ ∥) :=
+  fix go (apps : list E.term) (t : E.term) : typing_result bool:=
+    match t with
+    | E.tRel i => ret true
+    | E.tEvar ev args =>
+      res <- monad_map (go []) args ;;
+      ret (forallb id res)
+    | E.tLambda na M => go [] M
+    | E.tApp u v =>
+      b1 <- go (v :: apps) u ;;
+      b2 <- go [] v ;;
+      ret (b1 && b2)
+    | E.tLetIn na b b' =>
+      b1 <- go [] b;;
+      b2 <- go [] b';;
+      ret (b1 && b2)
+    | E.tCase ind c brs =>
+      b1 <- go [] c ;;
+      res <- monad_map (fun x => go [] (snd x)) brs ;;
+      ret (b1 && forallb id res)
+    | E.tProj p c => go [] c
+    | E.tFix mfix idx =>
+      res <- monad_map (fun x => go [] (E.dbody x)) mfix ;;
+      ret (forallb id res)
+    | E.tCoFix mfix idx =>
+      res <- monad_map (fun x => go [] (E.dbody x)) mfix ;;
+      ret (forallb id res)
+    | E.tBox => ret true
+    | E.tVar _ => ret true
+    | E.tConst nm => is_logargs_applied_const Σ HΣ nm (List.length apps)
+    | E.tConstruct ind i => ret true
+    end.
+
+Program Definition check_applied
+        (Σ : P.global_env)
+        (wf : ∥PCUICTyping.wf Σ∥)
+        (et : E.term) : EnvCheck bool :=
+  is_const_applied <- wrap_error (P.empty_ext Σ) "during checking applied constant"
+                                 (check_consts_applied (P.empty_ext Σ) _ [] et) ;;
+  let is_constr_applied := check_ctors_applied Σ [] et in
+  ret (Monad:=envcheck_monad) (andb is_const_applied is_constr_applied).
+Next Obligation. auto. Qed.
+
+Definition erase_and_check_applied (p : Ast.program) : EnvCheck bool :=
+  let p := fix_program_universes p in
+  let Σ := (trans_global (Ast.empty_ext p.1)).1 in
+  G <- check_wf_env_only_univs Σ ;;
+  et <- erase_template_program p ;;
+  check_applied Σ (proj2 (projT2 G)) et.2.
+
+Definition print_sum (s : string + string) :=
+  match s with
+  | inl s' => s'
+  | inr s' => s'
+  end.
+
+Definition opt_to_template {A} (o : option A) : TemplateMonad A:=
+  match o with
+  | Some v => ret v
+  | None => tmFail "None"
   end.
