extraction/theories/LiquidityExtract.v
@@ -1,0 +1,121 @@
+From Coq Require Import PeanoNat ZArith.
+
+From MetaCoq.Template Require Import Loader.
+From MetaCoq.Erasure Require Import SafeTemplateErasure.
+From MetaCoq.Erasure Require ErasureFunction.
+From MetaCoq.Erasure Require SafeErasureFunction.
+From MetaCoq.Template Require Import config.
+From MetaCoq.SafeChecker Require Import PCUICSafeReduce PCUICSafeChecker
+     SafeTemplateChecker.
+From MetaCoq.PCUIC Require Import PCUICAst PCUICAstUtils PCUICTyping
+     TemplateToPCUIC.
+
+From MetaCoq.Template Require Pretty.
+
+From ConCert.Execution Require Import Blockchain Serializable.
+
+From ConCert.Embedding Require Import MyEnv.
+From ConCert.Embedding Require Import Notations.
+From ConCert.Embedding Require Import SimpleBlockchain.
+
+From ConCert.Extraction Require Import LPretty
+     ExAst Erasure Optimize Common.
+
+From Coq Require Import List Ascii String.
+Local Open Scope string_scope.
+
+From MetaCoq.Template Require Import All.
+
+Import ListNotations.
+Import AcornBlockchain.
+Import MonadNotation.
+Import ResultMonad.
+
+Definition to_constant_decl (gd : option T.global_decl) :=
+  match gd with
+  | Some (ConstantDecl cst_body) => ret cst_body
+  | Some (InductiveDecl cst_body) => tmFail "Error (constant expected, given inductive)"
+  | None => tmFail "Error (expected constant with a body)"
+  end.
+
+Record LiquidityMod (msg init_ctx params storage operation : Type) :=
+  { lmd_module_name : string ;
+    lmd_prelude : string ;
+    lmd_init : init_ctx -> params -> option storage;
+    lmd_init_prelude : string ;
+    lmd_receive : msg -> storage -> option (list operation * storage);
+    lmd_entry_point : string }.
+
+Arguments lmd_module_name {_ _ _ _ _}.
+Arguments lmd_prelude {_ _ _ _ _}.
+Arguments lmd_init {_ _ _ _ _}.
+Arguments lmd_init_prelude {_ _ _ _ _}.
+Arguments lmd_receive {_ _ _ _ _}.
+Arguments lmd_entry_point {_ _ _ _ _}.
+
+
+Definition printLiquidityDefs (prefix : string) (Σ : global_env)
+           (TT : MyEnv.env string)
+           (ignore : list kername)
+           (build_call_ctx : string)
+           (init_prelude : string)
+           (init : kername)
+           (receive : kername)
+  : string + string :=
+  let seeds := [init;receive] in
+  match specialize_erase_debox_template_env Σ seeds ignore with
+  | Ok eΣ =>
+    (* dependencies should be printed before the dependent definitions *)
+    let ldef_list := List.rev (print_global_env prefix TT eΣ) in
+    (* filtering empty strings corresponding to the ignored definitions *)
+    let ldef_list := filter (negb ∘ (String.eqb "") ∘ snd) ldef_list in
+    match ExAst.lookup_env eΣ init with
+    | Some (ExAst.ConstantDecl init_cst) =>
+      match print_init prefix TT build_call_ctx init_prelude eΣ init_cst with
+      | Some init_code =>
+        (* filtering out the definition of [init] and projecting the code *)
+        let defs :=
+            map snd (filter (negb ∘ (eq_kername init) ∘ fst) ldef_list) in
+        let res :=
+            concat (nl ++ nl) (defs ++[ init_code ]) %list in
+        inl res
+      | None => inr "Error: Empty body for init"
+      end
+    | Some _ => inr "Error: init must be a constant"
+    | None => inr "Error: No init found"
+    end
+  | Err e => inr e
+  end.
+
+Definition liquidity_ignore_default :=
+  [<%% prod %%>].
+
+(* We assume the structure of the context from the [PreludeExt]:
+  current_time , sender_addr, sent_amount, acc_balance *)
+Definition liquidity_call_ctx :=
+  "(Current.time (),
+   (Current.sender (),
+   (Current.amount (),
+    Current.balance ())))".
+
+Definition liquitidy_extraction {msg ctx params storage operation : Type}
+           (prefix : string)
+           (TT_defs : list (kername *  string))
+           (TT_ctors : MyEnv.env string)
+           (m : LiquidityMod msg ctx params storage operation) :=
+  '(Σ,_) <- tmQuoteRecTransp m false ;;
+  init_nm <- extract_def_name m.(lmd_init);;
+  receive_nm <- extract_def_name m.(lmd_receive);;
+  let ignore := (map fst TT_defs ++ liquidity_ignore_default)%list in
+  let TT :=
+      (TT_ctors ++ map (fun '(kn,d) => (string_of_kername kn, d)) TT_defs)%list in
+  p <- tmEval lazy
+             (printLiquidityDefs prefix Σ TT ignore
+                                 liquidity_call_ctx
+                                 m.(lmd_init_prelude)
+                                 init_nm receive_nm) ;;
+  match p with
+  | inl s =>
+    tmEval lazy (concat (nl ++ nl) [m.(lmd_prelude); s; m.(lmd_entry_point)])
+  | inr s => tmFail s
+  end.
